add translation validation to UntypedComp5

src/UntypedComp5.v
@@ -3,6 +3,7 @@ Require Import Common.
 Require Import Utopia.
 Require Import Metadata.
 Require Import Program.
+Require Import Monads.
 
 Require Import ListLemmas.
 Require Import HList.
@@ -19,9 +20,21 @@ Module B := Untyped5.
 Module S := Untyped4.
 
 
-Definition compile_genv := @id (list S.expr).
+Section compile.
+Open Scope option_monad.
 
-Definition compile_cu := @id (list S.expr * list metadata)%type.
+Definition compile_genv (a : S.env) : option S.env :=
+    if A.no_values_list_dec a then
+        Some a
+    else
+        None.
+
+Definition compile_cu (cu : list S.expr * list metadata) : option (list S.expr * list metadata) :=
+    let '(exprs, metas) := cu in
+    compile_genv exprs >>= fun exprs' =>
+    Some (exprs', metas).
+
+End compile.
 
 
 
@@ -112,6 +125,7 @@ Qed.
 
 Theorem I_sim : forall E a a' b,
     Forall (fun e => ~ S.is_value e) E ->
+    A.cases_arent_values_state a ->
     I a b ->
     A.sstep E a a' ->
     exists b',
@@ -119,7 +133,7 @@ Theorem I_sim : forall E a a' b,
         I a' b'.
 
 destruct a as [ae l ak | v];
-intros0 Henv II Astep; inv Astep.
+intros0 Henv Acavs II Astep; inv Astep.
 all: inv II.
 
 all: try solve [eexists; split; repeat i_ctor].
@@ -135,17 +149,66 @@ all: try solve [eexists; split; repeat i_ctor].
 
 - eexists. split. left. i_lem B.SEliminate.
   i_ctor. eapply unroll_elim_not_value.
-  + admit. (* need cases_arent_values *)
+  + on >A.cases_arent_values_state, invc.
+    simpl in *.  A.refold_cases_arent_values.
+    repeat break_and.  rewrite A.cases_arent_values_list_is_Forall in *.
+    pattern case. i_lem Forall_nth_error.
   + intros. inversion 1.
 
-Admitted.
+Qed.
 
 
+Inductive I' : S.state -> S.state -> Prop :=
+| I'_intro : forall a b,
+        I a b ->
+        A.cases_arent_values_state a ->
+        I' a b.
+
+Theorem I'_sim : forall E a a' b,
+    Forall (fun e => ~ S.is_value e) E ->
+    Forall A.cases_arent_values E ->
+    I' a b ->
+    A.sstep E a a' ->
+    exists b',
+        (B.sstep E b b' \/ (b' = b /\ metric a' < metric a)) /\
+        I' a' b'.
+intros. on >I', invc.
+fwd eapply I_sim; eauto. break_exists; break_and.
+eexists; split; eauto. constructor; eauto.
+eapply A.step_cases_arent_values; try eassumption.
+Qed.
+
+
+
+Lemma compile_genv_eq : forall A B,
+    compile_genv A = Some B ->
+    A = B.
+simpl. inversion 1.
+unfold compile_genv in *. break_match; try discriminate.
+congruence.
+Qed.
 
 Lemma compile_cu_eq : forall A Ameta B Bmeta,
-    compile_cu (A, Ameta) = (B, Bmeta) ->
+    compile_cu (A, Ameta) = Some (B, Bmeta) ->
     A = B.
-simpl. inversion 1. auto.
+simpl. inversion 1. break_bind_option. inject_some.
+eauto using compile_genv_eq.
+Qed.
+
+Lemma compile_genv_no_values : forall A B,
+    compile_genv A = Some B ->
+    Forall A.no_values A.
+intros. unfold compile_genv in *.
+break_match; try discriminate.
+rewrite A.no_values_list_is_Forall in *.
+auto.
+Qed.
+
+Lemma compile_cu_no_values : forall A Ameta B Bmeta,
+    compile_cu (A, Ameta) = Some (B, Bmeta) ->
+    Forall A.no_values A.
+intros. simpl in *. break_bind_option.
+i_lem compile_genv_no_values.
 Qed.
 
 Section Preservation.
@@ -153,30 +216,35 @@ Section Preservation.
     Variable aprog : A.prog_type.
     Variable bprog : B.prog_type.
 
-    Hypothesis Hcomp : compile_cu aprog = bprog.
+    Hypothesis Hcomp : compile_cu aprog = Some bprog.
 
     Theorem fsim : Semantics.forward_simulation (A.semantics aprog) (B.semantics bprog).
     destruct aprog as [A Ameta], bprog as [B Bmeta].
     fwd eapply compile_cu_eq; eauto.
+    fwd eapply compile_cu_no_values; eauto.
 
     eapply Semantics.forward_simulation_star with
-        (match_states := I)
+        (match_states := I')
         (match_values := @eq value).
 
     - simpl. intros0 Bcall Hf Ha. invc Bcall.
       simpl in *.
       eexists. split; repeat i_ctor.
-      + admit. (* global env contains no values *)
+      + pattern body. eapply Forall_nth_error; try eassumption.
+        i_lem A.no_values_not_value_list.
+      + pattern body. eapply Forall_nth_error; try eassumption.
+        i_lem A.no_values_cases_arent_values_list.
 
-    - simpl. intros0 II Afinal. invc Afinal. invc II.
+    - simpl. intros0 II Afinal. invc Afinal. invc II. on >I, invc.
       eexists. split. i_ctor. i_ctor.
 
     - intros0 Astep. intros0 II.
       simpl in *. subst B.
-      eapply sstar_01_semantics_sim, I_sim; eauto.
-      + admit. (* global env contains no values *)
+      eapply sstar_01_semantics_sim, I'_sim; eauto.
+      + i_lem A.no_values_not_value_list.
+      + i_lem A.no_values_cases_arent_values_list.
 
-    Admitted.
+    Qed.
 
 End Preservation.
 
